Some initial experiments for encoding as nat with the lifting framework

Lib/Encode_Nat/Lifting_Nat.thy
@@ -1,24 +1,28 @@
 theory Lifting_Nat
-  imports Main "HOL-Library.Nat_Bijection" "HOL-Library.Simps_Case_Conv"
+  imports
+    Main
+    "HOL-Library.Nat_Bijection"
+    "HOL-Library.Simps_Case_Conv"
+    Encode_Nat
 begin
 
 section \<open>Lifting to \<^typ>\<open>nat\<close>\<close>
 
-class lift_nat =
+class lift_nat = order_bot +
   fixes Abs_nat :: "'a \<Rightarrow> nat"
   fixes Rep_nat :: "nat \<Rightarrow> 'a"
   assumes Rep_nat_Abs_nat_id[simp]: "\<And>x. Rep_nat (Abs_nat x) = x"
 begin
 
 lemma inj_Abs_nat: "inj Abs_nat"
-  using Rep_nat_Abs_nat_id unfolding inj_def by metis
+  by(rule inj_on_inverseI[of _ Rep_nat], simp)
 
 definition cr_nat :: "nat \<Rightarrow> 'a \<Rightarrow> bool" where
   "cr_nat \<equiv> (\<lambda>n l. n = Abs_nat l)"
 
 lemma typedef_nat: "type_definition Abs_nat Rep_nat (Abs_nat ` UNIV)"
   by (unfold_locales) auto
- 
+
 lemmas typedef_nat_transfer[OF typedef_nat cr_nat_def, transfer_rule] =
   typedef_bi_unique typedef_right_unique typedef_left_unique typedef_right_total
 
@@ -29,52 +33,54 @@ lemma cr_nat_Abs_nat[transfer_rule]:
 end
 
 
-abbreviation "fstP x \<equiv> fst (prod_decode x)"
-abbreviation "sndP x \<equiv> snd (prod_decode x)"
-
-
 section \<open>Lifting from \<^typ>\<open>bool\<close>\<close>
 
 instantiation bool :: lift_nat
 begin
 
-definition Abs_nat_bool_def: "Abs_nat b \<equiv> if b then 1 else 0"
+definition Abs_nat_bool_def:
+  "Abs_nat \<equiv> enc_bool"
 
-definition Rep_nat_bool_def: "Rep_nat n \<equiv> if n = 0 then False else True"
+definition Rep_nat_bool_def:
+  "Rep_nat \<equiv> dec_bool"
 
-instance 
-  apply (intro_classes)
-   apply (auto simp: Abs_nat_bool_def Rep_nat_bool_def)
-  done
+instance
+  by (intro_classes, simp add: Abs_nat_bool_def Rep_nat_bool_def enc_bool.simps True_nat_def
+      False_nat_def split: bool.split)
 
 end
 
 lemma Domainp_nat_bool_rel[transfer_domain_rule]:
-  "Domainp (cr_nat :: _ \<Rightarrow> bool \<Rightarrow> _) = (\<lambda>x. x = 0 \<or> x = 1)"
-  unfolding cr_nat_def Abs_nat_bool_def by auto
+  "Domainp (cr_nat :: _ \<Rightarrow> bool \<Rightarrow> _) = (\<lambda>x. x = False_nat \<or> x = True_nat)"
+  unfolding cr_nat_def Abs_nat_bool_def
+  by (auto simp add:  enc_bool.simps split:bool.split)
 
 context includes lifting_syntax
 begin
 
 \<comment> \<open>Needs to be provided by the datatype compiler\<close>
 lemma cr_nat_bool_True[transfer_rule]:
-  "cr_nat 1 True"
-  unfolding cr_nat_def Abs_nat_bool_def by auto
+  "cr_nat True_nat True"
+  unfolding cr_nat_def Abs_nat_bool_def
+  by(simp add: enc_bool.simps)
 
 \<comment> \<open>Needs to be provided by the datatype compiler\<close>
 lemma cr_nat_bool_False[transfer_rule]:
-  "cr_nat 0 False"
-  unfolding cr_nat_def Abs_nat_bool_def by auto
+  "cr_nat False_nat False"
+  unfolding cr_nat_def Abs_nat_bool_def
+  by(simp add: enc_bool.simps)
 
 lemma nat_bool_rel_conj[transfer_rule]:
   "(cr_nat ===> cr_nat ===> cr_nat) min (\<and>)"
   unfolding cr_nat_def Abs_nat_bool_def
-  by (auto simp: rel_fun_def)
+  by (simp add: rel_fun_def enc_bool.simps False_nat_def prod_encode_def split:bool.splits)
 
 lemma nat_bool_rel_disj[transfer_rule]:
   "(cr_nat ===> cr_nat ===> cr_nat) max (\<or>)"
   unfolding cr_nat_def Abs_nat_bool_def
-  by (auto simp: rel_fun_def)
+  by (simp add: rel_fun_def enc_bool.simps False_nat_def prod_encode_def split:bool.splits)
+
+term "(cr_nat ===> cr_nat) P_nat P"
 
 end
 
@@ -89,84 +95,25 @@ schematic_goal
 section \<open>Lifting from \<^typ>\<open>'a list\<close>\<close>
 
 \<comment> \<open>Already provided by the datatype compiler\<close>
-definition "case_list_nat f g xs \<equiv>
-  let
-    (t, as) = prod_decode xs
-  in
-    if t = 0
-      then f
-      else let (x, xs) = prod_decode as in g x xs
-"
 
-lemma case_list_nat_cong[fundef_cong]:
-  assumes "xs1 = xs2"
-  assumes "fstP xs2 = 0 \<Longrightarrow> f1 = f2"
-  assumes "fstP xs2 \<noteq> 0
-    \<Longrightarrow> g1 (fstP (sndP xs2)) (sndP (sndP xs2)) = g2 (fstP (sndP xs2)) (sndP (sndP xs2))"
-  shows "case_list_nat f1 g1 xs1 = case_list_nat f2 g2 xs2"
-  using assms unfolding case_list_nat_def
-  by (auto split: prod.splits simp: Let_def)
 
-lemma fst_prod_decode_aux_lt:
-  "0 < n \<Longrightarrow> fst (prod_decode_aux k n) < k + n"
-proof(induction k n rule: prod_decode_aux.induct)
-  case (1 k m)
-  then show ?case
-    apply (subst prod_decode_aux.simps)
-    apply simp
-    using prod_decode_aux.simps by fastforce
-qed
-
-lemma snd_prod_decode_aux_lt:
-  "1 < n \<Longrightarrow> snd (prod_decode_aux k n) < k + n"
-proof(induction k n rule: prod_decode_aux.induct)
-  case (1 k m)
-  then show ?case
-    apply (subst prod_decode_aux.simps)
-    apply simp
-    using prod_decode_aux.simps by fastforce
-qed
-
-lemma fstP_lt: "0 < n \<Longrightarrow> fstP n < n"
-  unfolding prod_decode_def using fst_prod_decode_aux_lt[where ?k=0] by simp
-
-lemma sndP_lt: "1 < n \<Longrightarrow> sndP n < n"
-  unfolding prod_decode_def using snd_prod_decode_aux_lt[where ?k=0] by simp
 
 instantiation list :: (lift_nat) lift_nat
 begin
 
-\<comment> \<open>Already provided by the datatype compiler\<close>
-fun Abs_nat_list :: "'a list \<Rightarrow> nat" where
-  "Abs_nat_list [] = prod_encode (0, 0)"
-| "Abs_nat_list (x # xs) =
-    prod_encode (1, prod_encode (Abs_nat x, Abs_nat_list xs))"
+definition "Abs_nat_list \<equiv> enc_list (Abs_nat :: 'a \<Rightarrow> nat)"
 
-\<comment> \<open>Already provided by the datatype compiler\<close>
-function Rep_nat_list :: "nat \<Rightarrow> 'a list" where
-  "Rep_nat_list n = case_list_nat [] (\<lambda>x xs. Rep_nat x # Rep_nat_list xs) n"
-  by auto
-termination
-proof -
-  have "0 < fstP n \<Longrightarrow> sndP (sndP n) < n" for n
-    apply (cases n) apply(auto)
-     apply (metis le_prod_encode_1 linorder_not_le prod.exhaust_sel prod_decode_inverse)
-    by (metis bot_nat_0.not_eq_extremum fstP_lt le_prod_encode_2 less_add_same_cancel1 not_less_eq
-        order_less_le_trans plus_1_eq_Suc prod.exhaust_sel prod_decode_inverse sndP_lt)
-  then show ?thesis
-    apply (relation "measure (\<lambda>n. size n)")
-     apply (auto)
-    done
-qed
-declare Rep_nat_list.simps[simp del]
+
+definition "Rep_nat_list \<equiv> dec_list (Rep_nat :: nat \<Rightarrow> 'a)"
+
+
 
 instance
-proof(intro_classes)
-  show "Rep_nat (Abs_nat xs) = xs" for xs :: "'a list"
-    apply (induction xs)
-     apply (subst Rep_nat_list.simps, simp add: case_list_nat_def)+
-    done
-qed
+  apply(intro_classes)
+  unfolding Rep_nat_list_def Abs_nat_list_def
+  using encoding_list_wellbehaved[THEN pointfree_idE] eq_id_iff
+  by fastforce
+
 
 end
 
@@ -189,27 +136,32 @@ begin
   each constructor.
 \<close>
 lemma cr_nat_list_Nil[transfer_rule]:
-  "cr_nat (prod_encode (0, 0)) []"
-  unfolding cr_nat_def by simp
+  "cr_nat (Nil_nat) []"
+  unfolding cr_nat_def Abs_nat_list_def
+  by(simp add: enc_list.simps Nil_nat_def)
 
 \<comment> \<open>Needs to be provided by the datatype compiler\<close>
 lemma cr_nat_list_Cons[transfer_rule]:
-  "(cr_nat ===> cr_nat ===> cr_nat) (\<lambda>x xs. prod_encode (1, prod_encode (x, xs))) (#)"
-  unfolding cr_nat_def by (auto simp: rel_fun_def)
+  "(cr_nat ===> cr_nat ===> cr_nat) Cons_nat (#)"
+  unfolding cr_nat_def Abs_nat_list_def
+  by (simp add: rel_fun_def enc_list.simps)
+
 
 \<comment> \<open>Needs to be provided by the datatype compiler\<close>
 lemma cr_nat_list_case_list[transfer_rule]:
   "(R ===> (cr_nat ===> cr_nat ===> R) ===> cr_nat ===> R) case_list_nat case_list"
-  unfolding cr_nat_def case_list_nat_def
-  by (auto simp: rel_fun_def split: prod.splits list.splits)
+  unfolding cr_nat_def case_list_nat_def Abs_nat_list_def
+  using case_list_eq_if
+  by (simp add: rel_fun_def Nil_nat_def Cons_nat_def enc_list.simps split: list.split)
 
 \<comment> \<open>Can be proved with Kevin's transport framework\<close>
+
 lemma rev_tr_nat_lifting[transfer_rule]:
   includes lifting_syntax
   shows "(cr_nat ===> cr_nat ===> cr_nat) (rev_tr_nat TYPE('a::lift_nat)) (rev_tr :: 'a list \<Rightarrow> _)"
   unfolding rev_tr_nat_def cr_nat_def
-  apply(auto simp: rel_fun_def)
-  done
+  by(simp add: rel_fun_def)
+
 
 end
 
@@ -228,12 +180,143 @@ lemma rev_tr_nat_synth_def:
   assumes "accn = Abs_nat acc"
   assumes "xsn = Abs_nat xs"
   shows "rev_tr_nat TYPE('a) accn xsn
-    = case_list_nat accn (\<lambda>x3a. rev_tr_nat TYPE('a) (prod_encode (1, prod_encode (x3a, accn)))) xsn"
+    = case_list_nat accn (\<lambda>x3a. rev_tr_nat TYPE('a) (Cons_nat x3a accn)) xsn"
   apply(rule HOL.trans[OF _ rev_tr_nat_synth[unfolded cr_nat_def, symmetric]])
-  apply(use assms in \<open>simp_all add: rev_tr_nat_def\<close>)
+    apply(use assms in \<open>simp_all add: rev_tr_nat_def\<close>)
   done
+
 
 \<comment> \<open>Final theorem that can be passed to the IMP compiler\<close>
 thm rev_tr_nat_synth_def[unfolded case_list_nat_def]
+
+
+fun elemof :: "'a \<Rightarrow> 'a list \<Rightarrow> bool" where
+  "elemof _ [] = False"
+| "elemof y (x#xs) = (if (y = x) then True else elemof y xs)"
+
+
+case_of_simps elemof_case_def: elemof.simps
+
+definition elemof_nat :: "'a::lift_nat itself \<Rightarrow> nat \<Rightarrow> nat \<Rightarrow> nat" where
+  "elemof_nat _ x xs \<equiv> (Abs_nat :: bool \<Rightarrow> nat) (elemof ((Rep_nat::nat => 'a) x) (Rep_nat xs))"
+
+lemma elemof_nat_lifting[transfer_rule]:
+  includes lifting_syntax
+  shows "(cr_nat ===> cr_nat ===> cr_nat) (elemof_nat TYPE('a::lift_nat)) (elemof :: 'a \<Rightarrow> _)"
+  unfolding elemof_nat_def cr_nat_def
+  by(simp add: rel_fun_def)
+
+
+schematic_goal elemof_nat_synth:
+  assumes [transfer_rule]: "(cr_nat :: nat \<Rightarrow> 'a \<Rightarrow> bool) xn (Rep_nat xn)"
+  assumes [transfer_rule]: "(cr_nat :: nat \<Rightarrow> 'a list \<Rightarrow> bool) xsn (Rep_nat xsn)"
+  shows "cr_nat ?t ((elemof :: 'a::lift_nat \<Rightarrow> _) (Rep_nat xn) (Rep_nat xsn))"
+  apply (subst elemof_case_def)
+  apply transfer_prover_start
+           apply transfer_step+
+  apply (rule HOL.refl)
+  done
+
+lemma elemof_nat_synth_def:
+  fixes x :: "'a::lift_nat " and xs :: "'a list"
+  assumes "xn = Abs_nat x"
+  assumes "xsn = Abs_nat xs"
+  shows "elemof_nat TYPE('a) xn xsn
+    = case_list_nat False_nat (\<lambda>y ys. if xn = y then True_nat else elemof_nat TYPE('a) xn ys) xsn"
+  apply(rule HOL.trans[OF _ elemof_nat_synth[unfolded cr_nat_def, symmetric]])
+    apply(use assms in \<open>simp_all add: elemof_nat_def\<close>)
+  done
+
+thm elemof_nat_synth_def[unfolded case_list_nat_def]
+
+definition If_nat :: "'a::lift_nat itself \<Rightarrow> nat \<Rightarrow> nat \<Rightarrow> nat \<Rightarrow> nat" where
+  "If_nat _ c t f \<equiv> (Abs_nat :: 'a \<Rightarrow> nat) (If (Rep_nat c) (Rep_nat t) (Rep_nat f))"
+
+definition case_bool_nat :: "nat \<Rightarrow> nat \<Rightarrow> nat \<Rightarrow> nat" where
+  "case_bool_nat t f c =
+  (if fstP c = atomic 1 then t else f)"
+
+lemma case_bool_nat_equiv:
+  "enc_'a (case_bool t f c) = case_bool_nat (enc_'a t) (enc_'a f) (enc_bool c)"
+  unfolding case_bool_nat_def
+  by(simp add: enc_bool.simps True_nat_def False_nat_def split: bool.split)
+
+lemma cr_nat_bool_case_bool[transfer_rule]:
+  includes lifting_syntax
+  shows "(cr_nat ===> cr_nat ===> cr_nat ===> cr_nat) case_bool_nat case_bool"
+  unfolding cr_nat_def case_bool_nat_def Abs_nat_bool_def
+  using case_bool_eq_if
+  by (simp add: rel_fun_def False_nat_def True_nat_def enc_bool.simps split: bool.split)
+
+
+lemma If_nat_lifting[transfer_rule]:
+  includes lifting_syntax
+  shows "(cr_nat ===> cr_nat ===> cr_nat ===> cr_nat)
+  (If_nat TYPE('a::lift_nat)) (If :: bool \<Rightarrow> 'a \<Rightarrow> 'a \<Rightarrow> 'a)"
+  by(simp add: If_nat_def rel_fun_def cr_nat_def)
+
+lemma If_case_def: "If c t f = (case c of True \<Rightarrow> t | False \<Rightarrow> f)" by simp
+
+schematic_goal If_nat_synth:
+  assumes [transfer_rule]: "(cr_nat :: nat \<Rightarrow> bool \<Rightarrow> bool) c (Rep_nat c)"
+  assumes [transfer_rule]: "(cr_nat :: nat \<Rightarrow> 'a \<Rightarrow> bool) t (Rep_nat t)"
+  assumes [transfer_rule]: "(cr_nat :: nat \<Rightarrow> 'a \<Rightarrow> bool) f (Rep_nat f)"
+  shows "cr_nat ?t ((If :: bool \<Rightarrow> 'a::lift_nat \<Rightarrow> 'a \<Rightarrow> 'a) (Rep_nat c) (Rep_nat t) (Rep_nat f))"
+  apply (subst If_case_def)
+  apply transfer_prover_start
+      apply transfer_step+
+  apply (rule HOL.refl)
+  done
+
+lemma If_nat_synth_def:
+  fixes c :: "bool" and t :: "'a::lift_nat" and f :: "'a"
+  assumes "cn = Abs_nat c"
+  assumes "tn = Abs_nat t"
+  assumes "fn = Abs_nat f"
+  shows "If_nat TYPE('a) cn tn fn = case_bool_nat tn fn cn"
+  apply(rule HOL.trans[OF _ If_nat_synth[unfolded cr_nat_def, symmetric]])
+  unfolding If_nat_def assms by simp+
+
+
+fun takeWhile :: "('a \<Rightarrow> bool) \<Rightarrow> 'a list \<Rightarrow> 'a list" where
+  "takeWhile P [] = []" |
+  "takeWhile P (x # xs) = (if P x then x # takeWhile P xs else [])"
+
+case_of_simps takeWhile_case_def: takeWhile.simps
+
+definition takeWhile_nat :: "'a::lift_nat itself \<Rightarrow> (nat \<Rightarrow> nat) \<Rightarrow> nat \<Rightarrow> nat" where
+  "takeWhile_nat _ P xs \<equiv> (Abs_nat :: 'a list \<Rightarrow> nat) (takeWhile (Rep_nat \<circ> P \<circ> Abs_nat) (Rep_nat xs))"
+
+lemma takeWhile_nat_lifting[transfer_rule]:
+  includes lifting_syntax
+  assumes "(cr_nat ===> cr_nat) P_nat P"
+  shows "(cr_nat ===> cr_nat) (takeWhile_nat TYPE('a::lift_nat) P_nat)
+  ((takeWhile :: ('a \<Rightarrow> bool) \<Rightarrow> 'a list \<Rightarrow> 'a list) P)"
+  using assms
+  by(simp add: takeWhile_nat_def rel_fun_def comp_def cr_nat_def)
+
+
+schematic_goal takeWhile_nat_synth:
+  includes lifting_syntax
+  assumes [transfer_rule]: "(cr_nat :: nat \<Rightarrow> 'a list \<Rightarrow> bool) xsn (Rep_nat xsn)"
+  assumes [transfer_rule]:"(cr_nat ===> cr_nat) P_nat P"
+  shows "cr_nat ?t ((takeWhile :: ('a::lift_nat \<Rightarrow> bool) \<Rightarrow> _) P (Rep_nat xsn))"
+  apply (subst takeWhile_case_def)
+  apply transfer_prover_start
+          apply transfer_step+
+  apply (rule HOL.refl)
+  done
+
+lemma takeWhile_nat_synth_def:
+  includes lifting_syntax
+  fixes P :: "'a::lift_nat \<Rightarrow> bool" and xs :: "'a list"
+  assumes "(cr_nat ===> cr_nat) P_nat P"
+  assumes "xsn = Abs_nat xs"
+  shows "takeWhile_nat TYPE('a) P_nat xsn
+    = case_list_nat Nil_nat (\<lambda>x3a x2ba. If_nat TYPE('a list) (P_nat x3a)
+          (Cons_nat x3a (takeWhile_nat TYPE('a) P_nat x2ba)) Nil_nat) xsn"
+  apply(rule HOL.trans[OF _ takeWhile_nat_synth[unfolded cr_nat_def, symmetric]])
+  using assms apply(simp add: takeWhile_nat_def rel_fun_def cr_nat_def)+
+  done
 
 end
